feat: BoolExprNat -> AIG

LeanSAT/Heap.lean
@@ -2,10 +2,22 @@ import LeanSAT.Reflect.Tactics.Reflect
 import Std.Data.HashMap
 open Std
 
+-- Missing Array theorems?
+theorem Array.push_get (as : Array α) (a : α) (h : i < (as.push a).size) : (as.push a)[i] = if _ : i < as.size then as[i] else a :=
+  sorry
+
+theorem Array.push_get_old (as : Array α) (a : α) (h : i < as.size) : (as.push a)[i]'(by simp; omega) = as[i] := by
+  simp [Array.push_get, h]
+
+theorem Array.push_get_size (as : Array α) (a : α) : (as.push a)[as.size] = a := by
+  simp [Array.push_get]
+
+
 inductive Decl where
+| const (b : Bool)
 | atom (idx : Nat)
 | gate (x y : Nat) (xpol ypol : Bool)
-deriving BEq, Hashable
+deriving BEq, Hashable, Repr
 
 inductive Cache.WF : Array Decl → HashMap Decl Nat → Prop where
 | empty : Cache.WF decls HashMap.empty
@@ -13,6 +25,8 @@ inductive Cache.WF : Array Decl → HashMap Decl Nat → Prop where
 | push_cache (h : Cache.WF decls cache) : Cache.WF (decls.push decl) (cache.insert decl decls.size)
 
 def Cache (decls : Array Decl) := { map : HashMap Decl Nat // Cache.WF decls map }
+
+def Cache.empty (decls : Array Decl) : Cache decl := ⟨HashMap.empty, WF.empty⟩
 
 def Cache.noUpdate (cache : Cache decls) : Cache (decls.push decl) :=
   ⟨cache.val, Cache.WF.push_id cache.property⟩
@@ -31,59 +45,71 @@ axiom Cache.find?_property {decls : Array Decl} {idx : Nat} (c : Cache decls) (d
     (h : c.find? decl = some idx) : decls[idx]'(Cache.find?_bounds c decl h) = decl
 
 def IsDag (decls : Array Decl) : Prop := ∀ i lhs rhs lpol rpol (h : i < decls.size), decls[i] = .gate lhs rhs lpol rpol → lhs < i ∧ rhs < i
+theorem IsDag.empty : IsDag #[] := by
+  intro i lhs rhs lpol rpol h
+  simp only [Array.size_toArray, List.length_nil] at h
+  omega
 
 structure Env where
   decls : Array Decl
   cache : Cache decls
   inv : IsDag decls
 
-def denote (x : Nat) (assign : List Bool) (env : Env) : Bool :=
-  go x assign env.decls env.inv
+def Env.empty : Env := { decls := #[], cache := Cache.empty #[], inv := IsDag.empty }
+
+structure Env.Entrypoint where
+  env : Env
+  start : Nat
+  inv : start < env.decls.size
+
+def Env.denote (entry : Env.Entrypoint) (assign : List Bool) : Bool :=
+  go entry.start entry.env.decls assign entry.inv entry.env.inv
 where
-  go (x : Nat) (assign : List Bool) (decls : Array Decl) (h : IsDag decls) :=
-    if h₁ : x < decls.size then
-      match h₂ : decls[x] with
-      | .atom b  => assign.getD b false
-      | .gate lhs rhs lpol rpol =>
-        have := h x _ _ _ _ h₁ h₂
-        let lval := go lhs assign decls h
-        let rval := go rhs assign decls h
-        xor lval lpol && xor rval rpol
-    else
-      true
+  go (x : Nat) (decls : Array Decl) (assign : List Bool) (h1 : x < decls.size) (h2 : IsDag decls) :=
+    match h3 : decls[x] with
+    | .const b => b
+    | .atom v => assign.getD v false
+    | .gate lhs rhs lpol rpol =>
+      have := h2 x _ _ _ _ h1 h3
+      let lval := go lhs decls assign (by omega) h2
+      let rval := go rhs decls assign (by omega) h2
+      xor lval lpol && xor rval rpol
 
--- Missing Array theorems?
-theorem Array.push_get (as : Array α) (a : α) (h : i < (as.push a).size) : (as.push a)[i] = if _ : i < as.size then as[i] else a :=
-  sorry
-
-theorem Array.push_get_old (as : Array α) (a : α) (h : i < as.size) : (as.push a)[i]'(by simp; omega) = as[i] := by
-  simp [Array.push_get, h]
-
-theorem Array.push_get_size (as : Array α) (a : α) : (as.push a)[as.size] = a := by
-  simp [Array.push_get]
-
-theorem denote.go_lt_push (x : Nat) (decls : Array Decl) (h1 : x < decls.size) {h2} {h3} (inv : IsDag decls) :
-    (denote.go x assign decls h2) = (denote.go x assign (decls.push decl) h3) := by
-  have h4 : x < decls.size + 1 := by omega
+theorem Env.denote.go_lt_push (x : Nat) (decls : Array Decl) (h1 : x < decls.size) {h2} {h3} (inv : IsDag decls) :
+    (denote.go x decls assign h1 h2) = (denote.go x (decls.push decl) assign (by simp; omega) h3) := by
   unfold denote.go
-  simp [h1, h4]
-  rw [Array.push_get_old]
+  simp [h1]
+  have h4 := Array.push_get_old decls decl h1
   split
   . next heq1 =>
-    rw [heq1]
-  . next lhs rhs lpol rpol heq1 =>
-    rw [heq1]
-    simp
-    have := inv x lhs rhs lpol rpol h1 heq1
-    apply ReflectSat.EvalAtAtoms.and_congr
+    split
     all_goals
-      apply ReflectSat.EvalAtAtoms.xor_congr
-      . apply denote.go_lt_push
-        omega
-        assumption
-      . rfl
+      next heq2 =>
+        rw [h4, heq1] at heq2;
+        injections
+  . next heq1 =>
+    split
+    . next heq2 => rw [h4, heq1] at heq2; injections
+    . next heq2 => rw [h4, heq1] at heq2; injection heq2 with heq3; simp [heq3]
+    . next heq2 => rw [h4, heq1] at heq2; injections
+  . next lhs1 rhs1 lpol1 rpol1 heq1 =>
+    split
+    . next heq2 => rw [h4, heq1] at heq2; injections
+    . next heq2 => rw [h4, heq1] at heq2; injections
+    . next lhs2 rhs2 lpol2 rpol2 heq2 =>
+      rw [heq1, heq2] at h4
+      injection h4 with lhseq rhseq lpoleq rpoleq
+      simp only [lhseq, lpoleq, rhseq, rpoleq]
+      have := inv x lhs1 rhs1 lpol1 rpol1 h1 heq1
+      apply ReflectSat.EvalAtAtoms.and_congr
+      all_goals
+        apply ReflectSat.EvalAtAtoms.xor_congr
+        . apply denote.go_lt_push
+          assumption
+        . rfl
 
-def mkGate (lhs rhs : Nat) (lpol rpol : Bool) (env : Env) (hl : lhs < env.decls.size) (hr : rhs < env.decls.size) : Nat × Env :=
+def Env.mkGate (lhs rhs : Nat) (lpol rpol : Bool) (env : Env) (hl : lhs < env.decls.size) 
+    (hr : rhs < env.decls.size) : Env.Entrypoint :=
   let g := env.decls.size
   let decls := env.decls.push (.gate lhs rhs lpol rpol)
   let cache := env.cache.noUpdate
@@ -93,13 +119,26 @@ def mkGate (lhs rhs : Nat) (lpol rpol : Bool) (env : Env) (hl : lhs < env.decls.
     split at h2
     . apply env.inv <;> assumption
     . injections; omega
-  (g, { env with decls, inv, cache })
+  ⟨{ env with decls, inv, cache }, g, by simp [g, decls]⟩
 
-def mkGateCache (lhs rhs : Nat) (lpol rpol : Bool) (env : Env) (hl : lhs < env.decls.size) (hr : rhs < env.decls.size) : Nat × Env :=
+theorem Env.mkGate_le_size (lhs rhs : Nat) (lpol rpol : Bool) (env : Env) hl hr
+    : env.decls.size ≤ (env.mkGate lhs rhs lpol rpol hl hr).env.decls.size := by
+  simp_arith [mkGate]
+
+theorem Env.lt_mkGate_size (e1 : Env.Entrypoint) (lhs rhs : Nat) (lpol rpol : Bool) hl hr
+    : e1.start < (e1.env.mkGate lhs rhs lpol rpol hl hr).env.decls.size := by
+  have h1 := e1.inv
+  have h2 : e1.env.decls.size ≤ (e1.env.mkGate lhs rhs lpol rpol hl hr).env.decls.size :=
+    Env.mkGate_le_size _ _ _ _ _ _ _
+  omega
+
+def Env.mkGateCached (lhs rhs : Nat) (lpol rpol : Bool) (env : Env) (hl : lhs < env.decls.size)
+    (hr : rhs < env.decls.size) : Env.Entrypoint :=
   let decl := .gate lhs rhs lpol rpol
-  if let some gate := env.cache.find? decl then
-    (gate, env)
-  else
+  match h:env.cache.find? decl with
+  | some gate =>
+    ⟨env, gate, by apply Cache.find?_bounds _ _ h⟩
+  | none =>
     let g := env.decls.size
     let decls := env.decls.push decl
     let cache := Cache.insert env.cache decl
@@ -110,37 +149,37 @@ def mkGateCache (lhs rhs : Nat) (lpol rpol : Bool) (env : Env) (hl : lhs < env.d
       split at h2
       . apply env.inv <;> assumption
       . injections; omega
-    (g, { env with decls, inv, cache })
+    ⟨{ env with decls, inv, cache }, g, by simp [g, decls]⟩
 
-theorem mkGateCache_eval_eq_mkGate_eval (lhs rhs : Nat) (lpol rpol : Bool) (env : Env) (hl : lhs < env.decls.size)
-    (hr : rhs < env.decls.size)
-    : let (g1, e1) := mkGateCache lhs rhs lpol rpol env hl hr
-      let (g2, e2) := mkGate lhs rhs lpol rpol env hl hr
-      denote g1 assign e1 = denote g2 assign e2 := by
-  simp only [mkGate, mkGateCache]
+theorem Env.mkGateCached_eval_eq_mkGate_eval (lhs rhs : Nat) (lpol rpol : Bool) (env : Env) (hl : lhs < env.decls.size)
+    (hr : rhs < env.decls.size) : denote (env.mkGateCached lhs rhs lpol rpol hl hr) assign = denote (env.mkGate lhs rhs lpol rpol hl hr) assign := by
+  simp only [mkGate, mkGateCached]
   split
   . next heq1 =>
     unfold denote denote.go
-    have h1 := Cache.find?_bounds env.cache (.gate lhs rhs lpol rpol) heq1
-    have h2 := Cache.find?_property env.cache (.gate lhs rhs lpol rpol) heq1
-    simp only [h1, Array.size_push, Nat.lt_succ_self, ↓reduceDite]
-    rw [Array.push_get_size]
+    have h1 := Cache.find?_property env.cache (.gate lhs rhs lpol rpol) heq1
+    simp only [Array.size_push, Nat.lt_succ_self]
     split
-    . next heq2 => simp [h2] at heq2
-    . simp_all
-      apply ReflectSat.EvalAtAtoms.and_congr
-      all_goals
-        apply ReflectSat.EvalAtAtoms.xor_congr
-        . rw [denote.go_lt_push]
-          assumption
-          exact env.inv
-        . rfl
+    . next heq2 => rw [h1] at heq2; injections
+    . next heq2 => rw [h1] at heq2; injections
+    . next heq2 =>
+      split
+      . next heq3 => rw [Array.push_get_size] at heq3; injections
+      . next heq3 => rw [Array.push_get_size] at heq3; injections
+      . next heq3 =>
+        rw [Array.push_get_size] at heq3;
+        injection heq3 with lhseq rhseq lpoleq rpoleq
+        simp only [lhseq, lpoleq, rhseq, rpoleq]
+        simp_all only [Decl.gate.injEq]
+        apply ReflectSat.EvalAtAtoms.and_congr
+        all_goals
+          apply ReflectSat.EvalAtAtoms.xor_congr
+          . rw [denote.go_lt_push]
+            exact env.inv
+          . rfl
   . simp [denote]
 
-theorem mkGate_lt : (mkGate lhs rhs lpol rpol env hx hy).1 < (mkGate lhs rhs lpol rpol env hx hy).2.decls.size := by
-  simp [mkGate]
-
-def mkAtom (n : Nat) (env : Env) : Nat × Env :=
+def Env.mkAtom (n : Nat) (env : Env) : Env.Entrypoint :=
   let g := env.decls.size
   let decls := env.decls.push (.atom n)
   let cache := env.cache.noUpdate
@@ -151,16 +190,21 @@ def mkAtom (n : Nat) (env : Env) : Nat × Env :=
     split at h2
     . apply env.inv <;> assumption
     . contradiction
-  (g, { decls, inv, cache })
+  ⟨{ decls, inv, cache }, g, by simp [g, decls]⟩
 
-def mkAtomCache (n : Nat) (env : Env) : Nat × Env :=
+theorem Env.mkAtom_le_size (env : Env) (var : Nat)
+    : env.decls.size ≤ (env.mkAtom var).env.decls.size := by
+  simp_arith [mkAtom]
+
+def Env.mkAtomCached (n : Nat) (env : Env) : Env.Entrypoint :=
   let decl := .atom n
-  if let some gate := env.cache.find? decl then
-    (gate, env)
-  else
+  match h:env.cache.find? decl with
+  | some gate =>
+    ⟨env, gate, by apply Cache.find?_bounds _ _ h⟩
+  | none =>
     let g := env.decls.size
-    let decls := env.decls.push (.atom n)
-    let cache := env.cache.noUpdate
+    let decls := env.decls.push decl
+    let cache := env.cache.insert decl
     have inv := by
       intro i lhs rhs lpol rpol h1 h2
       simp only [decls] at *
@@ -168,26 +212,247 @@ def mkAtomCache (n : Nat) (env : Env) : Nat × Env :=
       split at h2
       . apply env.inv <;> assumption
       . contradiction
-    (g, { decls, inv, cache })
+  ⟨{ decls, inv, cache }, g, by simp [g, decls]⟩
 
-theorem mkAtomCache_eval_eq_mkAtom_eval (var : Nat) (env : Env)
-    : let (g1, e1) := mkAtomCache var env
-      let (g2, e2) := mkAtom var env
-      denote g1 assign e1 = denote g2 assign e2 := by
-    simp only [mkAtom, mkAtomCache]
+theorem Env.mkAtomCached_eval_eq_mkAtom_eval (var : Nat) (env : Env)
+    : denote (env.mkAtomCached var) assign = denote (env.mkAtom var) assign := by
+  simp only [mkAtom, mkAtomCached]
+  split
+  . next heq1 =>
+    unfold denote denote.go
+    have h1 := Cache.find?_property env.cache (.atom var) heq1
+    simp only [Array.size_push, Nat.lt_succ_self]
     split
-    . next heq1 =>
-      unfold denote denote.go
-      have h1 := Cache.find?_bounds env.cache (.atom var) heq1
-      have h2 := Cache.find?_property env.cache (.atom var) heq1
-      simp only [h1, ↓reduceDite, Array.size_push, Nat.lt_succ_self]
-      rw [Array.push_get_size]
+    . next heq2 => rw [h1] at heq2; injections
+    . next heq2 =>
       split
-      . next heq2 =>
-        rw [h2] at heq2
-        injection heq2 with heq3
-        rw [heq3]
-      . next heq2 => 
-        rw [h2] at heq2
-        injection heq2
-    . simp [denote]
+      . next heq3 => rw [Array.push_get_size] at heq3; injections
+      . next heq3 =>
+        rw [Array.push_get_size] at heq3
+        rw [heq2] at h1
+        injections
+        simp [*]
+      . next heq3 => rw [Array.push_get_size] at heq3; injections
+    . next heq2 => rw [h1] at heq2; injections
+  . simp [denote]
+
+def Env.mkConst (val : Bool) (env : Env) : Env.Entrypoint :=
+  let g := env.decls.size
+  let decls := env.decls.push (.const val)
+  let cache := env.cache.noUpdate
+  have inv := by
+    intro i lhs rhs lpol rpol h1 h2
+    simp only [decls] at *
+    simp only [Array.push_get] at h2
+    split at h2
+    . apply env.inv <;> assumption
+    . contradiction
+  ⟨{ decls, inv, cache }, g, by simp [g, decls]⟩
+
+theorem Env.mkConst_le_size (env : Env) (val : Bool)
+    : env.decls.size ≤ (env.mkConst val).env.decls.size := by
+  simp_arith [mkConst]
+
+theorem Env.lt_mkConst_size (e1 : Env.Entrypoint) : e1.start < (e1.env.mkConst val).env.decls.size := by
+  have h1 := e1.inv
+  have h2 : e1.env.decls.size ≤ (e1.env.mkConst val).env.decls.size :=
+    Env.mkConst_le_size _ _
+  omega
+
+def Env.mkConstCached (val : Bool) (env : Env) : Env.Entrypoint :=
+  let decl := .const val
+  match h:env.cache.find? decl with
+  | some gate =>
+    ⟨env, gate, by apply Cache.find?_bounds _ _ h⟩
+  | none =>
+    let g := env.decls.size
+    let decls := env.decls.push decl
+    let cache := env.cache.insert decl
+    have inv := by
+      intro i lhs rhs lpol rpol h1 h2
+      simp only [decls] at *
+      simp only [Array.push_get] at h2
+      split at h2
+      . apply env.inv <;> assumption
+      . contradiction
+  ⟨{ decls, inv, cache }, g, by simp [g, decls]⟩
+
+theorem Env.mkConstCached_eval_eq_mkConst_eval (val : Bool) (env : Env)
+    : denote (env.mkConstCached val) assign = denote (env.mkConst val) assign := by
+  simp only [mkConst, mkConstCached]
+  split
+  . next heq1 =>
+    unfold denote denote.go
+    have h1 := Cache.find?_property env.cache (.const val) heq1
+    simp only [Array.size_push, Nat.lt_succ_self]
+    split
+    . next heq2 =>
+      split
+      . next heq3 =>
+        rw [Array.push_get_size] at heq3
+        rw [heq2] at h1
+        injection heq3 with heq4
+        rw [heq4] at h1
+        injections
+      . next heq3 => rw [Array.push_get_size] at heq3; injections
+      . next heq3 => rw [Array.push_get_size] at heq3; injections
+    . next heq2 => rw [h1] at heq2; injections
+    . next heq2 => rw [h1] at heq2; injections
+  . simp [denote]
+
+-- TODO: implement version of this with cached functions and prove equivalent
+def Env.ofBoolExprNat (expr : BoolExprNat) : Env.Entrypoint :=
+  go expr Env.empty
+where
+  go (expr : BoolExprNat) (env : Env) : { entry : Env.Entrypoint // env.decls.size ≤ entry.env.decls.size } :=
+    match expr with
+    | .literal var => ⟨env.mkAtom var, (by apply Env.mkAtom_le_size)⟩
+    | .const val => ⟨env.mkConst val, (by apply Env.mkConst_le_size)⟩
+    | .not expr =>
+      -- ¬x = true && invert x
+      let ⟨exprEntry, _⟩ := go expr env
+      let constEntry := exprEntry.env.mkConst true
+      have := exprEntry.env.mkConst_le_size true
+      let ret :=
+       constEntry.env.mkGate
+         constEntry.start
+         exprEntry.start
+         true
+         false
+         constEntry.inv
+         (by apply Env.lt_mkConst_size)
+      have := constEntry.env.mkGate_le_size _ _ true false constEntry.inv (by apply Env.lt_mkConst_size)
+      ⟨ret, by dsimp [constEntry, ret] at *; omega⟩
+    | .gate g lhs rhs =>
+      let ⟨lhsEntry, _⟩ := go lhs env
+      let ⟨rhsEntry, _⟩ := go rhs lhsEntry.env
+      have h1 : lhsEntry.start < Array.size rhsEntry.env.decls := by
+        have := lhsEntry.inv
+        omega
+      match g with
+      | .and =>
+        let ret :=
+          rhsEntry.env.mkGate
+            lhsEntry.start
+            rhsEntry.start
+            true
+            true
+            h1
+            rhsEntry.inv
+        have := rhsEntry.env.mkGate_le_size _ _ true true h1 rhsEntry.inv
+        ⟨ret, by dsimp [ret] at *; omega⟩
+      | .or =>
+        -- x or y = true && (invert (invert x && invert y))
+        let auxEntry :=
+          rhsEntry.env.mkGate
+            lhsEntry.start
+            rhsEntry.start 
+            false
+            false
+            h1
+            rhsEntry.inv
+        have := rhsEntry.env.mkGate_le_size _ _ false false h1 rhsEntry.inv
+        let constEntry := auxEntry.env.mkConst true
+        have := auxEntry.env.mkConst_le_size true
+        let ret :=
+          constEntry.env.mkGate
+            constEntry.start
+            auxEntry.start
+            true
+            false
+            constEntry.inv
+            (by apply Env.lt_mkConst_size)
+        have := constEntry.env.mkGate_le_size _ auxEntry.start true false constEntry.inv (by apply Env.lt_mkConst_size)
+        ⟨ret, by dsimp [auxEntry, constEntry, ret] at *; omega⟩
+      | .xor =>
+        -- x xor y = (invert (invert (x && y))) && (invert ((invert x) && (invert y)))
+        let aux1Entry :=
+          rhsEntry.env.mkGate
+            lhsEntry.start
+            rhsEntry.start
+            true
+            true
+            h1
+            rhsEntry.inv
+        have := rhsEntry.env.mkGate_le_size _ _ true true h1 rhsEntry.inv
+        have h3 : lhsEntry.start < aux1Entry.env.decls.size := by
+          dsimp [aux1Entry] at *
+          omega
+        let aux2Entry :=
+          aux1Entry.env.mkGate
+            lhsEntry.start
+            rhsEntry.start
+            false
+            false
+            h3
+            (by apply Env.lt_mkGate_size)
+        have := aux1Entry.env.mkGate_le_size _ _ false false h3 (by apply Env.lt_mkGate_size)
+        let ret :=
+          aux2Entry.env.mkGate
+            aux1Entry.start
+            aux2Entry.start
+            false
+            false
+            (by apply Env.lt_mkGate_size)
+            aux2Entry.inv
+        have := aux2Entry.env.mkGate_le_size aux1Entry.start _ false false (by apply Env.lt_mkGate_size) aux2Entry.inv
+        ⟨ret, by simp (config := { zetaDelta := true}) only at *; omega⟩
+      | .beq =>
+        -- a == b = (invert (a && (invert b))) && (invert ((invert a) && b))
+        let aux1Entry :=
+          rhsEntry.env.mkGate
+            lhsEntry.start
+            rhsEntry.start
+            true
+            false
+            h1
+            rhsEntry.inv
+        have := rhsEntry.env.mkGate_le_size _ _ true false h1 rhsEntry.inv
+        have h3 : lhsEntry.start < aux1Entry.env.decls.size := by
+          dsimp [aux1Entry] at *
+          omega
+        let aux2Entry :=
+          aux1Entry.env.mkGate
+            lhsEntry.start
+            rhsEntry.start
+            false
+            true
+            h3
+            (by apply Env.lt_mkGate_size)
+        have := aux1Entry.env.mkGate_le_size _ _ false true h3 (by apply Env.lt_mkGate_size)
+        let ret :=
+          aux2Entry.env.mkGate
+            aux1Entry.start
+            aux2Entry.start
+            false
+            false
+            (by apply Env.lt_mkGate_size)
+            aux2Entry.inv
+        have := aux2Entry.env.mkGate_le_size aux1Entry.start _ false false (by apply Env.lt_mkGate_size) aux2Entry.inv
+        ⟨ret, by simp (config := { zetaDelta := true}) only at *; omega⟩
+      | .imp =>
+        -- a -> b = true && (invert (a and (invert b)))
+        let auxEntry :=
+          rhsEntry.env.mkGate
+            lhsEntry.start
+            rhsEntry.start 
+            true
+            false
+            h1
+            rhsEntry.inv
+        have := rhsEntry.env.mkGate_le_size _ _ true false h1 rhsEntry.inv
+        let constEntry := mkConst true auxEntry.env
+        have := auxEntry.env.mkConst_le_size true
+        let ret :=
+          constEntry.env.mkGate
+            constEntry.start
+            auxEntry.start
+            true
+            false
+            constEntry.inv
+            (by apply Env.lt_mkConst_size)
+        have := constEntry.env.mkGate_le_size _ auxEntry.start true false constEntry.inv (by apply Env.lt_mkConst_size)
+        ⟨ret, by dsimp [auxEntry, constEntry, ret] at *; omega⟩
+
+
+#eval Env.ofBoolExprNat (.gate .and (.gate .and (.literal 0) (.literal 0)) (.gate .and (.literal 0) (.literal 0))) |>.env.decls
